src/lowparse/LowParse.Low.Combinators.fst
@@ -40,9 +40,10 @@ let validate_nochk32_nondep_then
   (#p2: parser k2 t2)
   (p2' : validator_nochk32 p2)
 : Tot (validator_nochk32 (nondep_then p1 p2))
-= fun (input: pointer buffer8) (len: pointer U32.t) ->
-  p1' input len;
-  p2' input len
+= fun (input: buffer8) ->
+  let off1 = p1' input in
+  let off2 = p2' (B.offset input off1) in
+  U32.add off1 off2
 
 inline_for_extraction
 let validate32_synth
@@ -71,8 +72,8 @@ let validate_nochk32_synth
     synth_injective f2
   })
 : Tot (validator_nochk32 (parse_synth p1 f2))
-= fun (input: pointer buffer8) (len: pointer U32.t) ->
-  p1' input len
+= fun (input: buffer8) ->
+  p1' input
 
 inline_for_extraction
 let validate32_total_constant_size
@@ -106,8 +107,11 @@ let validate_nochk32_constant_size
     k.parser_kind_low == U32.v sz
   })
 : Tot (validator_nochk32 p)
-= fun (input: pointer buffer8) (len: pointer U32.t) ->
-  advance_slice_ptr input len sz
+= fun (input: buffer8) ->
+  let h = HST.get () in
+  [@inline_let]
+  let _ = assert (Some? (parse p (B.as_seq h input))) in
+  sz
 
 inline_for_extraction
 let accessor_weaken
@@ -122,7 +126,7 @@ let accessor_weaken
   (rel': (t1 -> t2 -> GTot Type0))
   (u: unit { forall x1 x2 . rel x1 x2 ==> rel' x1 x2 } )
 : Tot (accessor p1 p2 rel')
-= fun input res -> a input res
+= fun input -> a input
 
 let rel_compose (#t1 #t2 #t3: Type) (r12: t1 -> t2 -> GTot Type0) (r23: t2 -> t3 -> GTot Type0) (x1: t1) (x3: t3) : GTot Type0 =
   exists x2 . r12 x1 x2 /\ r23 x2 x3
@@ -143,35 +147,39 @@ let accessor_compose
   (a12: accessor p1 p2 rel12)
   (a23: accessor p2 p3 rel23)
 : Tot (accessor p1 p3 (rel12 `rel_compose` rel23))
-= fun input res ->
-    a12 input res;
-    a23 input res
+= fun input ->
+    a23 (a12 input)
 
 inline_for_extraction
 let accessor_synth
   (#k: parser_kind)
   (#t1: Type)
   (#t2: Type)
-  (#p1: parser k t1)
-  (v1: validator_nochk32 p1)
+  (p1: parser k t1)
   (f: t1 -> GTot t2)
   (u: unit {  synth_injective f } )
 : Tot (accessor (parse_synth p1 f) p1 (fun x y -> f y == x))
-= fun input res -> truncate32 v1 input res
+= fun input ->
+  let h = HST.get () in
+  [@inline_let]
+  let _ = assert (Some? (parse p1 (B.as_seq h input))) in
+  input
 
 inline_for_extraction
 val nondep_then_fst
   (#k1: parser_kind)
   (#t1: Type0)
-  (#p1: parser k1 t1)
-  (p1' : validator_nochk32 p1)
+  (p1: parser k1 t1)
   (#k2: parser_kind)
   (#t2: Type0)
   (p2: parser k2 t2)
 : Tot (accessor (p1 `nondep_then` p2) p1 (fun x y -> y == fst x))
 
-let nondep_then_fst #k1 #t1 #p1 p1' #k2 #t2 p2 input sz =
-  truncate32 p1' input sz
+let nondep_then_fst #k1 #t1 p1 #k2 #t2 p2 input =
+  let h = HST.get () in
+  [@inline_let]
+  let _ = assert (Some? (parse p1 (B.as_seq h input))) in
+  input
 
 inline_for_extraction
 val nondep_then_snd
@@ -181,13 +189,11 @@ val nondep_then_snd
   (p1' : validator_nochk32 p1)
   (#k2: parser_kind)
   (#t2: Type0)
-  (#p2: parser k2 t2)
-  (p2' : validator_nochk32 p2)
+  (p2: parser k2 t2)
 : Tot (accessor (p1 `nondep_then` p2) p2 (fun x y -> y == snd x))
 
-let nondep_then_snd #k1 #t1 #p1 p1' #k2 #t2 #p2 p2' input sz =
-  p1' input sz;
-  truncate32 p2' input sz
+let nondep_then_snd #k1 #t1 #p1 p1' #k2 #t2 p2 input =
+  B.offset input (p1' input)
 
 inline_for_extraction
 let make_total_constant_size_parser32
@@ -205,9 +211,5 @@ let make_total_constant_size_parser32
       res == f (B.as_seq h s)
   ))))
 : Tot (parser32 (make_total_constant_size_parser sz t f))
-= fun (input: pointer buffer8) (len: pointer U32.t) ->
-  let b0 = B.index input 0ul in
-  let b = B.sub b0 0ul sz' in
-  let res = f' b in
-  advance_slice_ptr input len sz';
-  res
+= fun (input: buffer8) ->
+  f' (B.sub input 0ul sz')
