src/lowparse/LowParseExample3.Aux.fst
@@ -30,13 +30,13 @@ inline_for_extraction
 let access_a : accessor parse_t parse_u16 (fun x y -> y == x.a) =
   accessor_weaken (
     accessor_synth
-      ((validate_nochk32_u16 `validate_nochk32_nondep_then` validate_nochk32_u32) `validate_nochk32_nondep_then` validate_nochk32_u16)
+      ((parse_u16 `nondep_then` parse_u32) `nondep_then` parse_u16)
       synth_t
       ()
     `accessor_compose`
-    nondep_then_fst (validate_nochk32_u16 `validate_nochk32_nondep_then` validate_nochk32_u32) parse_u16
+    nondep_then_fst (parse_u16 `nondep_then` parse_u32) parse_u16
     `accessor_compose`
-    nondep_then_fst validate_nochk32_u16 parse_u32
+    nondep_then_fst parse_u16 parse_u32
   )
   (fun x y -> y == x.a) ()
 
@@ -44,13 +44,13 @@ inline_for_extraction
 let access_b : accessor parse_t parse_u32 (fun x y -> y == x.b) =
   accessor_weaken (
     accessor_synth
-      ((validate_nochk32_u16 `validate_nochk32_nondep_then` validate_nochk32_u32) `validate_nochk32_nondep_then` validate_nochk32_u16)
+      ((parse_u16 `nondep_then` parse_u32) `nondep_then` parse_u16)
       synth_t
       ()
     `accessor_compose`
-    nondep_then_fst (validate_nochk32_u16 `validate_nochk32_nondep_then` validate_nochk32_u32) parse_u16
+    nondep_then_fst (parse_u16 `nondep_then` parse_u32) parse_u16
     `accessor_compose`
-    nondep_then_snd validate_nochk32_u16 validate_nochk32_u32
+    nondep_then_snd validate_nochk32_u16 parse_u32
   )
   (fun x y -> y == x.b) ()
 
@@ -58,10 +58,10 @@ inline_for_extraction
 let access_c : accessor parse_t parse_u16 (fun x y -> y == x.c) =
   accessor_weaken (
     accessor_synth
-      ((validate_nochk32_u16 `validate_nochk32_nondep_then` validate_nochk32_u32) `validate_nochk32_nondep_then` validate_nochk32_u16)
+      ((parse_u16 `nondep_then` parse_u32) `nondep_then` parse_u16)
       synth_t
       ()
     `accessor_compose`
-    nondep_then_snd (validate_nochk32_u16 `validate_nochk32_nondep_then` validate_nochk32_u32) validate_nochk32_u16
+    nondep_then_snd (validate_nochk32_u16 `validate_nochk32_nondep_then` validate_nochk32_u32) parse_u16
   )
   (fun x y -> y == x.c) ()
